BB52Statement.v
@@ -15,12 +15,6 @@ Inductive Dir:Set :=
 | Dneg
 | Dpos.
 
-Definition Dir_rev(d:Dir) :=
-match d with
-| Dneg => Dpos
-| Dpos => Dneg
-end.
-
 Definition Dir_to_Z(x:Dir) :=
 match x with
 | Dneg => Zneg 1
