Sporadic_NonHalt.v
@@ -1,0 +1,95 @@
+From BusyCoq Require Import
+  Finned1 Finned2 Finned3 Finned4 Finned5
+  Skelet1 Skelet10 Skelet15 Skelet17 Skelet26 Skelet33 Skelet34 Skelet35.
+
+Definition tm_holdouts_13 :=
+  Finned1::Finned2::Finned3::Finned4::Finned5::
+  Skelet1::Skelet10::Skelet15::Skelet17::Skelet26::Skelet33::Skelet34::Skelet35::
+  nil.
+
+Lemma Finned1_nonhalt:
+  ~HaltsFromInit Σ Σ0 Finned1.
+Proof.
+  translate_nonhalt Finned1.tm Finned1.nonhalt.
+Qed.
+
+Lemma Finned2_nonhalt:
+  ~HaltsFromInit Σ Σ0 Finned2.
+Proof.
+  translate_nonhalt Finned2.tm Finned2.nonhalt.
+Qed.
+
+Lemma Finned3_nonhalt:
+  ~HaltsFromInit Σ Σ0 Finned3.
+Proof.
+  assert (H:~HaltsFromInit Σ Σ0 (to_TM Finned3.tm)) by (apply to_NonHalt,Finned3.nonhalt).
+  unfold HaltsFromInit in H.
+  unfold HaltsFromInit.
+  rewrite <-NonHalt_iff in H.
+  rewrite <-NonHalt_iff.
+  rewrite TM_to_rev_NF_spec in H.
+  replace (TM_to_rev_NF (to_TM Finned3.tm)) with Finned3 in H.
+  1: apply H.
+  fext. fext.
+  destruct x,x0; reflexivity.
+Qed.
+
+Lemma Finned4_nonhalt:
+  ~HaltsFromInit Σ Σ0 Finned4.
+Proof.
+  translate_nonhalt Finned4.tm Finned4.nonhalt.
+Qed.
+
+Lemma Finned5_nonhalt:
+  ~HaltsFromInit Σ Σ0 Finned5.
+Proof.
+  translate_nonhalt Finned5.tm Finned5.nonhalt.
+Qed.
+
+Lemma Skelet10_nonhalt:
+  ~HaltsFromInit Σ Σ0 Skelet10.
+Proof.
+  translate_nonhalt Skelet10.tm Skelet10.nonhalt.
+Qed.
+
+Lemma Skelet15_nonhalt:
+  ~HaltsFromInit Σ Σ0 Skelet15.
+Proof.
+  translate_nonhalt Skelet15.tm Skelet15.nonhalt.
+Qed.
+
+Lemma Skelet26_nonhalt:
+  ~HaltsFromInit Σ Σ0 Skelet26.
+Proof.
+  translate_nonhalt Skelet26.tm Skelet26.nonhalt.
+Qed.
+
+Lemma Skelet33_nonhalt:
+  ~HaltsFromInit Σ Σ0 Skelet33.
+Proof.
+  translate_nonhalt Skelet33.tm Skelet33.nonhalt.
+Qed.
+
+Lemma Skelet34_nonhalt:
+  ~HaltsFromInit Σ Σ0 Skelet34.
+Proof.
+  translate_nonhalt Skelet34.tm Skelet34.nonhalt.
+Qed.
+
+Lemma Skelet35_nonhalt:
+  ~HaltsFromInit Σ Σ0 Skelet35.
+Proof.
+  translate_nonhalt Skelet35.tm Skelet35.nonhalt.
+Qed.
+
+Lemma Skelet1_nonhalt:
+  ~HaltsFromInit Σ Σ0 Skelet1.
+Proof.
+  translate_nonhalt Skelet1.tm Skelet1.nonhalt.
+Qed.
+
+Lemma Skelet17_nonhalt:
+  ~HaltsFromInit Σ Σ0 Skelet17.
+Proof.
+  translate_nonhalt Skelet17.tm Skelet17.nonhalt.
+Qed.
